## Newton's first law of motion
- ==Newton's first law states that an object at rest tends to stay and rest and an object in motion tends to stay in motion unless acted upon by an unbalanced force==
### Inertia
- Inertia is the tendency of an object to continue it its original motion due to its mass
- Newton's first law is also known as the law of inertia
- Depends on the mass of an object; the greater the mass of a body, the higher its inertia -> the lesser it accelerates under the action of a given applied force
- Mass is a measure of inertia while weight is the gravitational force acting on a mass
## Linear momentum
- ==The linear momentum of an object is the product of the mass and the velocity==$$p=mv, p = Linear\ momentum (kg ms^{-1}), m = mass (kg), v = velocity (ms^{-1})$$
- Another unit for linear momentum is Newton Second ($Ns$ )
- A large object will have higher momentum than a smaller object
- An object moving at high velocity will have higher momentum than one moving with a lower velocity
## Newton's second law
- ==Newton's second law states that he rate of change of momentum is proportional to the net force acting on the object==, and this change in momentum takes place in the direction of the force$$F \propto \frac{d(mv)}{dt}$$
- Since we are using SI units, k, the constant is equal to 1
$$F = \frac{d(mv)}{dt} $$
- Applying chain rule,
$$F = m\frac{dv}{dt} + v\frac{dm}{dt} $$
- If the mass is constant, the rate of change of mass is 0 and $\frac{dv}{dt} = a$
$$F = m\frac{dv}{dt} = ma$$
- Hence, for a constant mass, $$F = ma, F =Force (N), m = mass (kg), a  =acceleration (kgms^{-2})$$
## Impulse
- For a variable force over a time interval, the area under the force-time graph is equivalent to the impulse
- The impulse is *equal in magnitude*  to the change in momentum
$$ Change\ in\ momentum\ \Delta p = Impulse\ I\ = Area\ under\ f-t\ graph $$
- This give us the impulse momentum theorem which states that the impulse of the force acting on the object is equal to the change in momentum of the object
## Newton's third law
- ==Newton's third law states that if body A exerts a force on body B, then body will exert and equal and opposite force on body A==
- The reaction force is equal in magnitude and opposite in direction to the original force
- The force acts on two different objects, so they do not cancel
### Weightlessness 
- Weightlessness refers to being in a state of free fall in which there is no perceived support (i.e. No reaction force on the person given by any support)
- The actual weight of the person is determined by his mass and the acceleration of gravity
- But one's perceived weight comes from that the fact that they are supported by a support
- People experience weightlessness if
	- An elevator cable breaks
	- Going over the top of a roller coaster
	- Putting an aircraft "over the hump" in ballistic trajectory
	- Being in orbit
## Principle of conservation of momentum
- ==The principle of conservation of momentum states that the total momentum of the system before the collision is equal to the total momentum of the system after the collision, provided no net external force acts on the system==$$m_a U_a + m_b U_b = m_a V_a + m_b V_b, m = mass (kg), U = initial\ velocity (ms^{-1}), V = final\ velocity (ms^{-1})$$$$ Total\ momentum\ before = Total\ momentum\ after$$
### Proof
- Consider Mass $A$ travelling with velocity $U_a$ collides with mass $B$ with velocity $U_b$ 
- During the collision, the two masses are in contact and exert a force F on each other, and the time of impact is T
- By Newton's second law ($F \propto \frac{d(mv)}{dt}$)
	- A: $F_A = M_A(V_A-U_A)/t$
	- B: $F_B = M_B(V_B-U_B)/t$
- By newton's third law (action has a reaction)
	- $F_B = -F_A$
	- $M_B(V_B-U_B)/t = -  M_A(V_A-U_A)/t$
- Rearranging,
	- $m_a U_a + m_b U_b = m_a V_a + m_b V_b$

## Elastic collisions
- An elastic collision is one where the total momentum is conserved, and the total kinetic energy is conserved
- An inelastic collision is one where the total momentum is conserved, and the total kinetic energy is not conserved
- For both collisions, total energy is conserved
- For an elastic collision, we can deduce that$$ U_1 - U_2 = V_2 - V_1, U = initial\ velocity\ (ms^{-1}),  V = final\ velocity\ (ms^{-1})$$
### Proof
- Conservation of momentum: $m_1 U_1 + m_2 U_2 = m_1 V_1 + m_2 V_2$
- Rearranging: $m_1(U_1-V_1) = m_2(U_2-V_2)$
- Conservation of kinetic energy: $\frac{1}{2}(m_1)(U_1)^2 +\frac{1}{2}(m_2)(U_2)^2$
- Rearranging: 